Choice.v
@@ -1,0 +1,4 @@
+Require Export Bigop.
+
+
+Check 1.
